Foundation/Modal/Kripke/AxiomWeakDot3.lean
@@ -1,0 +1,153 @@
+import Foundation.Modal.Kripke.Completeness
+
+
+
+namespace LO.Modal
+
+namespace Kripke
+
+section definability
+
+open Formula.Kripke
+
+variable {F : Kripke.Frame}
+
+lemma weakConnected_of_validate_WeakDot3 (hCon : WeakConnected F) : F ⊧ (Axioms.WeakDot3 (.atom 0) (.atom 1)) := by
+  rintro V x;
+  apply Satisfies.or_def.mpr;
+  suffices
+    (∀ (y : F.World), x ≺ y → V y 0 → (∀ (x : F.World), y ≺ x → V x 0) → V y 1) ∨
+    (∀ (y : F.World), x ≺ y → V y 1 → (∀ (x : F.World), y ≺ x → V x 1) → V y 0)
+    by simpa [Semantics.Realize, Satisfies];
+  by_contra hC;
+  push_neg at hC;
+  obtain ⟨⟨y, Rxy, hy0, hz, nhy1⟩, ⟨z, Rxz, hz1, hy, nhz0⟩⟩ := hC;
+  have nyz : y ≠ z := by
+    by_contra hC;
+    subst hC;
+    contradiction;
+  rcases hCon ⟨Rxy, Rxz, nyz⟩ with (Ryz | Rzy);
+  . have := hz _ Ryz; contradiction;
+  . have := hy _ Rzy; contradiction;
+
+lemma validate_WeakDot3_of_weakConnected : F ⊧ (Axioms.WeakDot3 (.atom 0) (.atom 1)) → WeakConnected F := by
+  contrapose;
+  intro hCon;
+  obtain ⟨x, y, Rxy, z, Rxz, nyz, nRyz, nRzy⟩ := by simpa [WeakConnected] using hCon;
+  apply ValidOnFrame.not_of_exists_valuation_world;
+  use (λ w a => match a with | 0 => w = y ∨ y ≺ w | 1 => w = z ∨ z ≺ w | _ => True), x;
+  suffices
+    ∃ w, x ≺ w ∧ (w = y ∨ y ≺ w) ∧ (∀ (v : F.World), w ≺ v → ¬v = y → y ≺ v) ∧ ¬w = z ∧ ¬z ≺ w ∧
+    ∃ w, x ≺ w ∧ (w = z ∨ z ≺ w) ∧ (∀ (v : F.World), w ≺ v → ¬v = z → z ≺ v) ∧ ¬w = y ∧ ¬y ≺ w by
+    simpa [Semantics.Realize, Satisfies];
+  refine ⟨
+    _,
+    Rxy,
+    by tauto,
+    by tauto,
+    by tauto,
+    nRzy,
+    _,
+    Rxz,
+    by tauto,
+    by tauto,
+    by tauto,
+    nRyz
+  ⟩;
+
+abbrev WeakConnectedFrameClass : FrameClass := { F | WeakConnected F }
+
+instance : WeakConnectedFrameClass.IsNonempty := by
+  use ⟨Unit, λ _ _ => True⟩;
+  simp [WeakConnected];
+
+instance WeakConnectedFrameClass.DefinedByWeakDot3 : WeakConnectedFrameClass.DefinedBy {Axioms.WeakDot3 (.atom 0) (.atom 1)} := ⟨by
+  intro F;
+  constructor;
+  . simpa using weakConnected_of_validate_WeakDot3;
+  . simpa using validate_WeakDot3_of_weakConnected;
+⟩
+
+end definability
+
+
+section canonicality
+
+variable {S} [Entailment (Formula ℕ) S]
+variable {𝓢 : S} [Entailment.Consistent 𝓢] [Entailment.K 𝓢]
+
+open Formula.Kripke
+open Entailment
+open MaximalConsistentTableau
+open canonicalModel
+
+namespace Canonical
+
+lemma weakConnected [Entailment.HasAxiomWeakDot3 𝓢] : WeakConnected (canonicalFrame 𝓢).Rel := by
+  rintro x y z ⟨Rxy, Rxz, eyz⟩;
+  by_contra hC;
+  push_neg at hC;
+  rcases hC with ⟨nRyz, nRzy⟩;
+
+  obtain ⟨φ₁, hφ₁y, hφ₁z⟩ := Set.not_subset.mp nRyz;
+  replace hφ₁y : □φ₁ ∈ y.1.1 := by simpa using hφ₁y;
+  replace hφ₁z : φ₁ ∈ z.1.2 := iff_not_mem₁_mem₂.mp hφ₁z;
+  obtain ⟨φ₂, hφ₂y, hφ₂z⟩ := exists₁₂_of_ne eyz;
+  let φ := φ₁ ⋎ φ₂;
+
+  obtain ⟨ψ₁, hψz, hψy⟩ := Set.not_subset.mp nRzy;
+  replace hψ₁z : □ψ₁ ∈ z.1.1 := by simpa using hψz;
+  replace hψ₁y : ψ₁ ∈ y.1.2 := iff_not_mem₁_mem₂.mp hψy;
+  obtain ⟨ψ₂, hψ₂z, hψ₂y⟩ := exists₂₁_of_ne eyz;
+  let ψ := ψ₁ ⋎ ψ₂;
+
+  apply x.neither (φ := □(⊡φ ➝ ψ) ⋎ □(⊡ψ ➝ φ));
+  constructor;
+  . exact iff_provable_mem₁.mp axiomWeakDot3! x;
+  . apply iff_mem₂_or.mpr;
+    constructor;
+    . apply iff_mem₂_box.mpr;
+      use y;
+      constructor;
+      . assumption;
+      . apply iff_mem₂_imp.mpr;
+        constructor;
+        . apply iff_mem₁_and.mpr;
+          constructor;
+          . apply iff_mem₁_or.mpr; tauto;
+          . apply iff_mem₁_box.mpr
+            intro u Ryu;
+            apply iff_mem₁_or.mpr;
+            left;
+            exact Ryu hφ₁y;
+        . apply iff_mem₂_or.mpr;
+          constructor;
+          . assumption;
+          . assumption;
+    . apply iff_mem₂_box.mpr;
+      use z;
+      constructor;
+      . assumption;
+      . apply iff_mem₂_imp.mpr;
+        constructor;
+        . apply iff_mem₁_and.mpr;
+          constructor;
+          . apply iff_mem₁_or.mpr; tauto;
+          . apply iff_mem₁_box.mpr
+            intro u Rzu;
+            apply iff_mem₁_or.mpr;
+            left;
+            exact Rzu hψ₁z;
+        . apply iff_mem₂_or.mpr;
+          constructor;
+          . assumption;
+          . assumption;
+
+end Canonical
+
+end canonicality
+
+
+end Kripke
+
+end LO.Modal
