Foundation/Modal/Kripke/Hilbert/K4Dot2.lean
@@ -1,0 +1,36 @@
+import Foundation.Modal.Kripke.AxiomWeakDot2
+import Foundation.Modal.Kripke.Hilbert.K4
+
+namespace LO.Modal
+
+open Kripke
+open Geachean
+
+
+abbrev Kripke.TransitiveWeakConfluentFrameClass : FrameClass := { F | Transitive F ∧ WeakConfluent F }
+
+instance Kripke.TransitiveWeakConfluentFrameClass.DefinedByK4Dot2Axioms
+  : FrameClass.DefinedBy Kripke.TransitiveWeakConfluentFrameClass Hilbert.K4Dot2.axioms := by
+  rw [
+    (show TransitiveWeakConfluentFrameClass = TransitiveFrameClass ∩ WeakConfluentFrameClass by aesop),
+    (show Hilbert.K4Dot2.axioms = Hilbert.K4.axioms ∪ {Axioms.WeakDot2 (.atom 0) (.atom 1)} by aesop)
+  ];
+  exact FrameClass.definedBy_inter Kripke.TransitiveFrameClass (Hilbert.K4.axioms) WeakConfluentFrameClass {Axioms.WeakDot2 (.atom 0) (.atom 1)};
+
+instance : Kripke.TransitiveWeakConfluentFrameClass.IsNonempty := by
+  use ⟨Unit, λ _ _ => True⟩;
+  simp [Reflexive, Transitive, WeakConfluent ];
+
+namespace Hilbert.K4Dot2
+
+instance Kripke.sound : Sound (Hilbert.K4Dot2) (TransitiveWeakConfluentFrameClass) := inferInstance
+
+instance Kripke.consistent : Entailment.Consistent (Hilbert.K4Dot2) := Hilbert.consistent_of_FrameClass TransitiveWeakConfluentFrameClass
+
+instance Kripke.canonical : Canonical (Hilbert.K4Dot2) (TransitiveWeakConfluentFrameClass) := ⟨Canonical.transitive, Canonical.weakConfluent⟩
+
+instance Kripke.complete : Complete (Hilbert.K4Dot2) (TransitiveWeakConfluentFrameClass) := inferInstance
+
+end Hilbert.K4Dot2
+
+end LO.Modal
